concurrency/hack-hash-table/MultisetLemmas.i.dfy
@@ -3,23 +3,32 @@ include "../../lib/Base/Multisets.i.dfy"
 module MultisetLemmas {
   import opened Multisets
 
-  lemma ApplyId<A>(fn: A ~> A, s: multiset<A>)
+  lemma ApplyId<A>(fn: A -> A, s: multiset<A>)
   requires forall x | x in s :: fn(x) == x
   ensures Apply(fn, s) == s
   {
   }
 
-  lemma ApplyCompose<A,B,C>(fn: A ~> B, gn: B ~> C, hn: A ~> C, s: multiset<A>)
+  lemma ApplyCompose<A,B,C>(fn: A -> B, gn: B -> C, hn: A -> C, s: multiset<A>)
   requires forall x | x in s :: gn(fn(x)) == hn(x)
   ensures Apply(gn, Apply(fn, s)) == Apply(hn, s)
   {
   }
 
-  lemma ApplyGetBackwards<A,B>(fn : A ~> B, s: multiset<A>, b: B)
+  lemma ApplyGetBackwards<A,B>(fn : A -> B, s: multiset<A>, b: B)
   returns (a: A)
   requires b in Apply(fn, s)
   ensures fn(a) == b
   ensures a in s
+  {
+  }
+
+  lemma apply_eq_1_2<A, B, C>(s: multiset<A>,
+      a_c: A -> C,
+      a_b: A -> B,
+      b_c: B -> C)
+  requires forall x | x in s :: a_c(x) == b_c(a_b(x))
+  ensures Apply(a_c, s) == Apply(b_c, Apply(a_b, s))
   {
   }
 }
